tweak logrel, define new tran_rel

theories/logrel/logrel.v
@@ -27,16 +27,16 @@ Section logrel.
       full entries.
       Pagetable entries are transferred along as both sender and receiver could be the exclusive owner of those pages. *)
   Definition transaction_pagetable_entries_transferred i (trans: gmap Addr transaction) : iProp Σ:=
-    big_sepFM trans (λ kv, kv.2.1.2 = Donation ∧ (kv.2.1.1.1.2 = i ∨ kv.2.1.1.1.1 = i)) (λ k v, k -{1/2}>t v.1 ∗ pgt v.1.1.2 1 v.1.1.1.1 true)%I.
+    big_sepFM trans (λ kv, kv.2.1.2 = Donation ∧ (kv.2.1.1.1.2 = i ∨ kv.2.1.1.1.1 = i)) (λ k v, k -{1/4}>t v.1 ∗ pgt v.1.1.2 1 v.1.1.1.1 true)%I.
 
   (* [retrieval entries]: half of all retrieval entries of i-related transactions are required.
      For transactions where i is the sender, we need the corresponding retrieval entries to check if it is allowed for i to reclaim,
      for the cases when i is the receiver, they are required so that i can retrieve or relinquish *)
   (* There are also some cases when we need the second half, as in those cases we may update/remove the retrival state *)
   (* XXX: How to relate retrieval and transaction entries? Using option(frac_agree transaction,option bool)? or is it unnecessary? *)
-  Definition retrieval_entries_transferred i (trans: gmap Addr transaction) : iProp Σ:=
+  Definition retrievable_transaction_transferred i (trans: gmap Addr transaction) : iProp Σ:=
     (big_sepFM trans (λ kv, kv.2.1.1.1.2 = i ∨ kv.2.1.1.1.1 = i) (λ k v, k -{1/2}>re v.2 )%I) ∗
-    (big_sepFM trans (λ kv, (kv.2.1.1.1.1 = i ∨ kv.2.1.1.1.2 = i) ∧ kv.2.2 = false) (λ k v, k -{1/2}>re v.2)%I).
+    (big_sepFM trans (λ kv, (kv.2.1.1.1.1 = i ∨ kv.2.1.1.1.2 = i) ∧ kv.2.2 = false) (λ k v, k -{1/4}>t v.1 ∗ k -{1/2}>re v.2)%I).
 
   (* [transaction_pagetable_entries_owned]: transaction and page table entries that are owned initially by i,
      i.e. they are not transferred by VMProp, so we doesn't need to take care of them when reasoning the primary VM.
@@ -46,20 +46,20 @@ Section logrel.
      while the sender needs full to reclaim, we let i always own half and only pass the otner half around with VMProp*)
   (* [TODO] relation to [pagetable_entries_excl_owned] *)
   Definition transaction_pagetable_entries_owned i (trans: gmap Addr transaction) : iProp Σ:=
-    big_sepFM trans (λ kv, kv.2.1.1.1.1 = i ∧ kv.2.1.2 ≠ Donation) (λ k v, k -{1/2}>t v.1 ∗ pgt v.1.1.2 1 v.1.1.1.1 (bool_decide (v.1.2 ≠ Sharing)))%I.
-
-  (* [TODO] *)
-  Definition retrieval_entries_owned i (trans: gmap Addr transaction) : iProp Σ:=
-    (big_sepFM trans (λ kv, kv.2.1.1.1.2 = i ∧ kv.2.2 = true) (λ k v, k -{1/2}>re v.2)%I).
-
-  Definition transaction_pagetable_entries_transferred_except (i: VMID) (trans: gmap Addr transaction) : iProp Σ:=
-    big_sepFM trans (λ kv, kv.2.1.2 = Donation ∧ ¬(kv.2.1.1.1.2 = i ∨ kv.2.1.1.1.1 = i)) (λ k v, k -{1/2}>t v.1 ∗ pgt v.1.1.2 1 v.1.1.1.1 true)%I.
-
-  Definition retrieval_entries_transferred_except (i: VMID) (trans: gmap Addr transaction) : iProp Σ:=
-    (big_sepFM trans (λ kv, ¬(kv.2.1.1.1.2 = i ∨ kv.2.1.1.1.1 = i)) (λ k v, k -{1/2}>re v.2 )%I) ∗
-    (big_sepFM trans (λ kv, ¬(kv.2.1.1.1.2 = i ∨ kv.2.1.1.1.1 = i) ∧ kv.2.2 = false) (λ k v, k -{1/2}>re v.2)%I).
+    big_sepFM trans (λ kv, kv.2.1.1.1.1 = i ∧ kv.2.1.2 ≠ Donation) (λ k v, k -{1/4}>t v.1 ∗ pgt v.1.1.2 1 v.1.1.1.1 (bool_decide (v.1.2 ≠ Sharing)))%I.
 
   Context (i : (leibnizO VMID)).
+
+  (* [TODO] *)
+  Definition retrieved_transaction_owned i (trans: gmap Addr transaction) : iProp Σ:=
+    (big_sepFM trans (λ kv, kv.2.1.1.1.2 = i ∧ kv.2.2 = true) (λ k v, k -{1/4}>t v.1 ∗ k -{1/2}>re v.2)%I).
+
+  (* Definition transaction_pagetable_entries_transferred_except (i: VMID) (trans: gmap Addr transaction) : iProp Σ:= *)
+  (*   big_sepFM trans (λ kv, kv.2.1.2 = Donation ∧ ¬(kv.2.1.1.1.2 = i ∨ kv.2.1.1.1.1 = i)) (λ k v, k -{1/2}>t v.1 ∗ pgt v.1.1.2 1 v.1.1.1.1 true)%I. *)
+
+  (* Definition retrieval_entries_transferred_except (i: VMID) (trans: gmap Addr transaction) : iProp Σ:= *)
+  (*   (big_sepFM trans (λ kv, ¬(kv.2.1.1.1.2 = i ∨ kv.2.1.1.1.1 = i)) (λ k v, k -{1/2}>re v.2 )%I) ∗ *)
+  (*   (big_sepFM trans (λ kv, ¬(kv.2.1.1.1.2 = i ∨ kv.2.1.1.1.1 = i) ∧ kv.2.2 = false) (λ k v, k -{1/2}>re v.2)%I). *)
 
   Program Definition interp_execute: iPropO Σ :=
    (⌜i ≠ V0⌝ -∗
@@ -88,6 +88,10 @@ Section logrel.
   Definition accessible_in_trans_memory_pages (trans : gmap Word transaction) :=
     pages_in_trans (filter (λ kv, (kv.2.1.1.1.1 = i  ∧ ¬(kv.2.2 = true ∧ kv.2.1.2 = Lending)) ∨ kv.2.1.1.1.2 = i) trans).
 
+  (* [currently_accessible_in_trans_memory_pages] currently accessible memory pages associated with transactions *)
+  Definition currently_accessible_in_trans_memory_pages (trans : gmap Word transaction) :=
+    pages_in_trans (filter (λ kv, (kv.2.1.1.1.1 = i  ∧ kv.2.1.2 = Sharing) ∨ (kv.2.1.1.1.2 = i ∧ kv.2.2 = true)) trans).
+
   (* [TODO] *)
   Definition rx_pages (s: gset VMID) : iProp Σ :=
     [∗ set] j ∈ s, ∃ p_rx, RX@ j := p_rx ∗ ∃ rx_state, RX_state{1/2}@j := rx_state ∗
@@ -100,13 +104,13 @@ Section logrel.
     (R0 @@ V0 ->r encode_hvc_func(Send) ∗ (∃ rx_state'', RX_state@ i := rx_state'') ∗ ∃ j p_rx l, ⌜j ≠ i⌝ ∗ RX@ j := p_rx ∗ RX_state{1/2}@j := Some(l,i)
                           ∗ (∃r1, R1 @@ V0 ->r r1 ∗ ⌜decode_vmid r1 = Some j⌝) ∗  R2 @@ V0 ->r l ∗ ∃ mem_rx, memory_page p_rx mem_rx).
 
-  Definition trans_rel (P : gmap Word transaction -d> iPropO Σ) (trans trans': gmap Word transaction ): iProp Σ:=
-    □(P trans -∗ P trans').
+  (* Definition trans_rel (P : gmap Word transaction -d> iPropO Σ) (trans trans': gmap Word transaction ): iProp Σ:= *)
+  (*   □(P trans -∗ P trans'). *)
 
-  Notation "t -{{ P }}∗ t'"  := (trans_rel P t t') ( at level 70, format "t  -{{ P }}∗  t'").
+  (* Notation "t -{{ P }}∗ t'"  := (trans_rel P t t') ( at level 70, format "t  -{{ P }}∗  t'"). *)
 
-  Definition vmprop_zero_pre (Ψ: PID -d> PID -d> (gmap Word transaction) -d> iPropO Σ) :PID -d> PID -d> (gmap Word transaction) -d> iPropO Σ :=
-    λ p_tx p_rx trans', (∃ ps_na'' ps_acc'' trans'' ,
+  Definition vmprop_zero_pre (Ψ: PID -d> PID -d> iPropO Σ) :PID -d> PID -d> iPropO Σ :=
+    λ p_tx p_rx, (∃ ps_na'' ps_acc'' trans'',
                            let ps_macc_trans'' := (transferred_memory_pages trans'') in
                            (* lower bound *)
                            i -@{1/2}A> ps_acc'' ∗
@@ -115,7 +119,7 @@ Section logrel.
                            (* transaction and pagetable entries *)
                            transaction_hpool_global_transferred trans'' ∗
                            transaction_pagetable_entries_transferred i trans'' ∗
-                           retrieval_entries_transferred i trans'' ∗
+                           retrievable_transaction_transferred i trans'' ∗
                            (* memory *)
                            (∃ mem_trans, memory_pages ps_macc_trans'' mem_trans) ∗
                            (* status of RX *)
@@ -123,23 +127,21 @@ Section logrel.
                            rx_page i p_rx ∗ (∃ mem_rx, memory_page p_rx mem_rx) ∗
                            rx_pages ((list_to_set (list_of_vmids)) ∖ {[i]}) ∗
                            return_reg_rx i ∗
-                           (* TODO: implications, to be proved later.. *)
+                           (* XXX: implications, to be proved later.. or not?? *)
                            (* (trans' -{{(transaction_pagetable_entries_transferred_except i)}}∗ trans'') ∗ *)
                            (* (trans' -{{(retrieval_entries_transferred_except i)}}∗ trans'') ∗ *)
                            (* (trans' -{{(transaction_pagetable_entries_owned V0)}}∗ trans'') ∗ *)
-                           VMProp i (Ψ p_tx p_rx trans'') (1/2)%Qp)%I.
+                           VMProp i (Ψ p_tx p_rx) (1/2)%Qp)%I.
 
   Definition vmprop_unknown_pre
-    (Φ: PID -d> PID -d> (gmap Word transaction) -d> iPropO Σ)
-    :PID -d> PID -d> (gmap Word transaction) -d> iPropO Σ :=
-    λ p_tx p_rx trans,
+    (Φ: PID -d> PID -d> iPropO Σ)
+    :PID -d> PID -d> iPropO Σ :=
+    λ p_tx p_rx,
     (∃ ps_na' ps_acc' (trans' : gmap Word transaction) rx_state,
-               let ps_macc_trans := (transferred_memory_pages trans) in
                let ps_macc_trans' := (transferred_memory_pages trans') in
                (* [ps_oea], we exclude all pages involved in in-flight transactions,
                 NOTE: it has to be (accessible_in_trans_memory_pages), ps_macc_trans doesn't make sense(even if we can complete the FTLR proof)*)
-               let ps_oea := ps_acc' ∖ {[p_rx;p_tx]} ∖ (accessible_in_trans_memory_pages trans) in
-               let ps_oea' := ps_acc' ∖ {[p_rx;p_tx]} ∖ (accessible_in_trans_memory_pages trans') in
+               (* let ps_oea' := ps_acc' ∖ {[p_rx;p_tx]} ∖ (currently_accessible_in_trans_memory_pages trans') in *)
                (* lower bound *)
                i -@{1/2}A> ps_acc' ∗
                LB@ i := [ps_na'] ∗
@@ -151,7 +153,7 @@ Section logrel.
                (* transaction and pagetable entries *)
                transaction_hpool_global_transferred trans' ∗
                transaction_pagetable_entries_transferred i trans' ∗
-               retrieval_entries_transferred i trans' ∗
+               retrievable_transaction_transferred i trans' ∗
                (* memory *)
                (∃ mem_trans, memory_pages ps_macc_trans' mem_trans) ∗
                R0 @@ V0 ->r encode_hvc_func(Run) ∗ R1 @@ V0 ->r encode_vmid(i) ∗ (∃ r2, R2 @@ V0 ->r r2) ∗
@@ -171,19 +173,20 @@ Section logrel.
                 in a concrete example(as we give a concrete [trans] at the first and can reason about what should be the
                 [trans'] that satisfies the relation as we know the behaviors of VMs) than in a general case. So we leave
                 the proofs to the users of LR. *)
-               ⌜ps_oea = ps_oea'⌝ ∗ ⌜retrieved_lending_memory_pages trans = retrieved_lending_memory_pages trans' ⌝ ∗
                (* ((∃ mem_oea, memory_pages ps_oea mem_oea) ∗ (∃ mem_trans, memory_transferred trans' mem_trans) -∗ *)
                (*  ∃ mem_all, memory_pages (ps_acc' ∖ {[p_rx;p_tx]} ∪ ps_macc_trans') mem_all) ∗ *)
                (* (pagetable_entries_excl_owned i ps_oea -∗ pagetable_entries_excl_owned i ps_oea') ∗ *)
-               (trans -{{transaction_pagetable_entries_owned i}}∗ trans') ∗
-               (trans -{{retrieval_entries_owned i}}∗ trans') ∗
+               (* TODO derive below with trans_rel *)
+               (* ⌜ps_oea = ps_oea'⌝ ∗ ⌜retrieved_lending_memory_pages trans = retrieved_lending_memory_pages trans' ⌝ ∗ *)
+               (* (trans -{{transaction_pagetable_entries_owned i}}∗ trans') ∗ *)
+               (* (trans -{{retrieval_entries_owned i}}∗ trans') ∗ *)
                (* if i yielding, we give following resources back to pvm *)
-               VMProp V0 (vmprop_zero_pre Φ p_tx p_rx trans') (1/2)%Qp)%I.
+               VMProp V0 (vmprop_zero_pre Φ p_tx p_rx) (1/2)%Qp)%I.
 
   Local Instance vmprop_unknown_pre_contractive : Contractive (vmprop_unknown_pre).
   Proof.
-    rewrite /vmprop_unknown_pre => n vmprop_unknown vmprop_unknown' Hvmprop_unknown p_tx p_rx trans /=.
-    do 26 f_equiv.
+    rewrite /vmprop_unknown_pre => n vmprop_unknown vmprop_unknown' Hvmprop_unknown p_tx p_rx /=.
+    do 22 f_equiv.
     rewrite /VMProp  /=.
     do 6 f_equiv.
     f_contractive.
@@ -191,7 +194,6 @@ Section logrel.
     do 17 f_equiv.
     rewrite /VMProp.
     repeat f_equiv.
-    apply Hvmprop_unknown.
   Qed.
 
   Definition vmprop_unknown:= fixpoint (vmprop_unknown_pre).
@@ -199,59 +201,55 @@ Section logrel.
   Definition vmprop_zero := vmprop_zero_pre vmprop_unknown.
 
   Lemma vmprop_unknown_def : vmprop_unknown ≡
-    λ p_tx p_rx trans,
+    λ p_tx p_rx,
       (∃ ps_na' ps_acc' (trans' : gmap Word transaction) rx_state,
-          let ps_macc_trans := (transferred_memory_pages trans) in
           let ps_macc_trans' := (transferred_memory_pages trans') in
-          let ps_oea := ps_acc' ∖ {[p_rx;p_tx]} ∖ (accessible_in_trans_memory_pages trans) in
-          let ps_oea' := ps_acc' ∖ {[p_rx;p_tx]} ∖ (accessible_in_trans_memory_pages trans') in
+          (* let ps_oea' := ps_acc' ∖ {[p_rx;p_tx]} ∖ (accessible_in_trans_memory_pages trans') in *)
           i -@{1/2}A> ps_acc' ∗
           LB@ i := [ps_na'] ∗
           ⌜ps_na' ## ps_acc' ∪ (accessible_in_trans_memory_pages trans')⌝ ∗
           transaction_hpool_global_transferred trans' ∗
           transaction_pagetable_entries_transferred i trans' ∗
-          retrieval_entries_transferred i trans' ∗
+          retrievable_transaction_transferred i trans' ∗
           (∃ mem_trans, memory_pages ps_macc_trans' mem_trans) ∗
           R0 @@ V0 ->r encode_hvc_func(Run) ∗ R1 @@ V0 ->r encode_vmid(i) ∗ (∃ r2, R2 @@ V0 ->r r2) ∗
           RX_state@ i := rx_state ∗
           (rx_page i p_rx) ∗
           (∃ mem_rx, memory_page p_rx mem_rx) ∗
           rx_pages (list_to_set (list_of_vmids) ∖ {[i]}) ∗
-          ⌜ps_oea = ps_oea'⌝ ∗ ⌜retrieved_lending_memory_pages trans = retrieved_lending_memory_pages trans' ⌝ ∗
-          (trans -{{transaction_pagetable_entries_owned i}}∗ trans') ∗
-          (trans -{{retrieval_entries_owned i}}∗ trans') ∗
-          VMProp V0 (vmprop_zero p_tx p_rx trans') (1/2)%Qp)%I.
+          (* ⌜ps_oea = ps_oea'⌝ ∗ ⌜retrieved_lending_memory_pages trans = retrieved_lending_memory_pages trans' ⌝ ∗ *)
+          (* (trans -{{transaction_pagetable_entries_owned i}}∗ trans') ∗ *)
+          (* (trans -{{retrieval_entries_owned i}}∗ trans') ∗ *)
+          VMProp V0 (vmprop_zero p_tx p_rx) (1/2)%Qp)%I.
   Proof.
     rewrite /vmprop_unknown //.
     rewrite (fixpoint_unfold vmprop_unknown_pre).
     setoid_reflexivity.
   Qed.
 
-  Global Instance vmprop_unknown_proper: Proper ((=) ==> (=) ==> (=) ==> (⊣⊢)) vmprop_unknown.
+  Global Instance vmprop_unknown_proper: Proper ((=) ==> (=) ==> (⊣⊢)) vmprop_unknown.
   Proof. apply _. Qed.
 
-  Lemma vmprop_unknown_eq (p_tx p_rx:PID) (trans: gmap Word transaction): vmprop_unknown p_tx p_rx trans ⊣⊢
+  Lemma vmprop_unknown_eq (p_tx p_rx:PID) : vmprop_unknown p_tx p_rx ⊣⊢
       (∃ ps_na' ps_acc' (trans' : gmap Word transaction) rx_state,
-               let ps_macc_trans := (transferred_memory_pages trans) in
                let ps_macc_trans' := (transferred_memory_pages trans') in
-               let ps_oea := ps_acc' ∖ {[p_rx;p_tx]} ∖ (accessible_in_trans_memory_pages trans) in
-               let ps_oea' := ps_acc' ∖ {[p_rx;p_tx]} ∖ (accessible_in_trans_memory_pages trans') in
+               (* let ps_oea' := ps_acc' ∖ {[p_rx;p_tx]} ∖ (accessible_in_trans_memory_pages trans') in *)
                i -@{1/2}A> ps_acc' ∗
                LB@ i := [ps_na'] ∗
                ⌜ps_na' ## ps_acc' ∪ (accessible_in_trans_memory_pages trans')⌝ ∗
                transaction_hpool_global_transferred trans' ∗
                transaction_pagetable_entries_transferred i trans' ∗
-               retrieval_entries_transferred i trans' ∗
+               retrievable_transaction_transferred i trans' ∗
                (∃ mem_trans, memory_pages ps_macc_trans' mem_trans) ∗
                R0 @@ V0 ->r encode_hvc_func(Run) ∗ R1 @@ V0 ->r encode_vmid(i) ∗ (∃ r2, R2 @@ V0 ->r r2) ∗
                RX_state@ i := rx_state ∗
                (rx_page i p_rx) ∗
                (∃ mem_rx, memory_page p_rx mem_rx) ∗
                rx_pages (list_to_set (list_of_vmids) ∖ {[i]}) ∗
-               ⌜ps_oea = ps_oea'⌝ ∗ ⌜retrieved_lending_memory_pages trans = retrieved_lending_memory_pages trans' ⌝ ∗
-               (trans -{{transaction_pagetable_entries_owned i}}∗ trans') ∗
-               (trans -{{retrieval_entries_owned i}}∗ trans') ∗
-               VMProp V0 (vmprop_zero p_tx p_rx trans') (1/2)%Qp)%I.
+               (* ⌜ps_oea = ps_oea'⌝ ∗ ⌜retrieved_lending_memory_pages trans = retrieved_lending_memory_pages trans' ⌝ ∗ *)
+               (* (trans -{{transaction_pagetable_entries_owned i}}∗ trans') ∗ *)
+               (* (trans -{{retrieval_entries_owned i}}∗ trans') ∗ *)
+               VMProp V0 (vmprop_zero p_tx p_rx) (1/2)%Qp)%I.
     Proof.
       rewrite /vmprop_unknown.
       (* be patient, this line takes 30+ sec.. *)
@@ -262,7 +260,7 @@ Section logrel.
     (
       (* exclusively owned pages are pages i has access to, but ain't in any transactions related to i. *)
       let ps_macc_trans := (transferred_memory_pages trans) in
-      let ps_oea := ps_acc ∖ {[p_rx;p_tx]} ∖ (accessible_in_trans_memory_pages trans) in
+      let ps_oea := ps_acc ∖ {[p_rx;p_tx]} ∖ (currently_accessible_in_trans_memory_pages trans) in
       (* registers *)
       (∃ regs, ⌜is_total_gmap regs⌝ ∗ [∗ map] r ↦ w ∈ regs, r @@ i ->r w) ∗
       (* TX page and its memory *)
@@ -272,11 +270,19 @@ Section logrel.
       ⌜{[p_tx;p_rx]} ⊆ ps_acc⌝ ∗
       pagetable_entries_excl_owned i ps_oea ∗
       transaction_pagetable_entries_owned i trans ∗
-      retrieval_entries_owned i trans ∗
+      retrieved_transaction_owned i trans ∗
       (∃ mem_oea, memory_pages (ps_oea ∪ (retrieved_lending_memory_pages trans)) mem_oea) ∗
-      VMProp i (vmprop_unknown p_tx p_rx trans) (1/2)%Qp
+      VMProp i (vmprop_unknown p_tx p_rx) (1/2)%Qp
     )%I.
 
+  Definition tran_rel_secondary (i:VMID) (trans trans': gmap Word transaction): Prop :=
+   map_Forall (λ h tran,
+       match tran with
+        | (sndr, rcvr, _, ty, retri) =>
+            ((sndr = i ∧ ty ≠ Donation) -> ∃ tran', trans' !! h = Some tran' ∧ tran.1 = tran'.1) ∧
+            ((rcvr = i ∧ retri = true) -> ∃ tran', trans' !! h = Some tran' ∧ tran = tran')
+       end
+     ) trans.
 End logrel.
 
 Section logrel_prim.
@@ -285,33 +291,43 @@ Section logrel_prim.
   Context `{hypparams:!HypervisorParameters}.
   Context `{vmG: !gen_VMG Σ}.
 
-  Definition transaction_pagetable_entries_transferred_all (trans: gmap Addr transaction) : iProp Σ:=
-    big_sepFM trans (λ kv, kv.2.1.2 = Donation) (λ k v, k -{1/2}>t v.1 ∗ pgt v.1.1.2 1 v.1.1.1.1 true)%I.
+  Definition tran_rel_primary (i:VMID) (trans trans': gmap Word transaction): Prop :=
+   map_Forall (λ h tran,
+       match tran with
+         | (sndr, rcvr, _, ty, retri) =>
+          ((sndr ≠ i ∧ rcvr ≠ i) -> ∃ tran', trans' !! h = Some tran' ∧ tran = tran') ∧
+          ((sndr = i ∧ retri = true) -> ∃ tran', trans' !! h = Some tran' ∧ tran = tran') ∧
+          ((rcvr = i ∧ ty ≠ Donation) -> ∃ tran', trans' !! h = Some tran' ∧ tran.1 = tran'.1)
+       end
+     ) trans.
 
-  Definition retrieval_entries_transferred_all(trans: gmap Addr transaction) : iProp Σ:=
-    (big_sepFM trans (λ kv, True) (λ k v, k -{1/2}>re v.2 )%I) ∗
-    (big_sepFM trans (λ kv, kv.2.2 = false) (λ k v, k -{1/2}>re v.2)%I).
+  (* Definition transaction_pagetable_entries_transferred_all (trans: gmap Addr transaction) : iProp Σ:= *)
+  (*   big_sepFM trans (λ kv, kv.2.1.2 = Donation) (λ k v, k -{1/2}>t v.1 ∗ pgt v.1.1.2 1 v.1.1.1.1 true)%I. *)
 
-  Program Definition interp_access_prim p_tx p_rx ps_acc trans rx_state: iPropO Σ:=
-    (
-      let ps_macc_trans := (transferred_memory_pages V0 trans) in
-      let ps_oea := ps_acc ∖ {[p_rx;p_tx]} ∖ (accessible_in_trans_memory_pages V0 trans) in
-      (∃ regs, ⌜is_total_gmap regs⌝ ∗ [∗ map] r ↦ w ∈ regs, r @@ V0 ->r w) ∗
-      (tx_page V0 p_tx ∗ ∃ mem_tx, memory_page p_tx mem_tx) ∗
-      V0 -@A> ps_acc ∗
-      ⌜{[p_tx;p_rx]} ⊆ ps_acc⌝ ∗
-      pagetable_entries_excl_owned V0 ps_oea ∗
-      transaction_pagetable_entries_owned V0 trans ∗ transaction_hpool_global_transferred trans ∗
-      transaction_pagetable_entries_transferred_all trans ∗
-      retrieval_entries_owned V0 trans ∗ retrieval_entries_transferred_all trans ∗
-      (∃ mem_oea, memory_pages ps_oea mem_oea) ∗
-      (∃ mem_trans, memory_pages ps_macc_trans mem_trans) ∗
-      RX_state@ V0 := rx_state ∗ (rx_page V0 p_rx) ∗
-      (∃ mem_rx, memory_page p_rx mem_rx) ∗
-      rx_pages (list_to_set (list_of_vmids) ∖ {[V0]}) ∗
-      VMProp V0 True 1%Qp ∗
-      [∗ set] i ∈ list_to_set (list_of_vmids) ∖ {[V0]}, VMProp (i:VMID) (vmprop_unknown i p_tx p_rx trans) (1/2)%Qp
-    )%I.
+  (* Definition retrieval_entries_transferred_all(trans: gmap Addr transaction) : iProp Σ:= *)
+  (*   (big_sepFM trans (λ kv, True) (λ k v, k -{1/2}>re v.2 )%I) ∗ *)
+  (*   (big_sepFM trans (λ kv, kv.2.2 = false) (λ k v, k -{1/2}>re v.2)%I). *)
+
+  (* Program Definition interp_access_prim p_tx p_rx ps_acc trans rx_state: iPropO Σ:= *)
+  (*   ( *)
+  (*     let ps_macc_trans := (transferred_memory_pages V0 trans) in *)
+  (*     let ps_oea := ps_acc ∖ {[p_rx;p_tx]} ∖ (accessible_in_trans_memory_pages V0 trans) in *)
+  (*     (∃ regs, ⌜is_total_gmap regs⌝ ∗ [∗ map] r ↦ w ∈ regs, r @@ V0 ->r w) ∗ *)
+  (*     (tx_page V0 p_tx ∗ ∃ mem_tx, memory_page p_tx mem_tx) ∗ *)
+  (*     V0 -@A> ps_acc ∗ *)
+  (*     ⌜{[p_tx;p_rx]} ⊆ ps_acc⌝ ∗ *)
+  (*     pagetable_entries_excl_owned V0 ps_oea ∗ *)
+  (*     transaction_pagetable_entries_owned V0 trans ∗ transaction_hpool_global_transferred trans ∗ *)
+  (*     transaction_pagetable_entries_transferred_all trans ∗ *)
+  (*     retrieved_transaction_owned V0 trans ∗ retrieval_entries_transferred_all trans ∗ *)
+  (*     (∃ mem_oea, memory_pages ps_oea mem_oea) ∗ *)
+  (*     (∃ mem_trans, memory_pages ps_macc_trans mem_trans) ∗ *)
+  (*     RX_state@ V0 := rx_state ∗ (rx_page V0 p_rx) ∗ *)
+  (*     (∃ mem_rx, memory_page p_rx mem_rx) ∗ *)
+  (*     rx_pages (list_to_set (list_of_vmids) ∖ {[V0]}) ∗ *)
+  (*     VMProp V0 True 1%Qp ∗ *)
+  (*     [∗ set] i ∈ list_to_set (list_of_vmids) ∖ {[V0]}, VMProp (i:VMID) (vmprop_unknown i p_tx p_rx) (1/2)%Qp *)
+  (*   )%I. *)
 
 End logrel_prim.
 
