theories/logrel/ftlr_nop.v
@@ -11,7 +11,7 @@ Section ftlr_nop.
   Context `{hypparams:!HypervisorParameters}.
   Context `{vmG: !gen_VMG Σ}.
 
-Lemma ftlr_nop {i trans' mem_acc_tx ai regs ps_acc p_tx p_rx ps_na instr} trans rx_state:
+Lemma ftlr_nop {i mem_acc_tx ai regs ps_acc p_tx p_rx ps_na instr} trans rx_state:
   base_extra.is_total_gmap regs ->
   {[p_tx; p_rx]} ⊆ ps_acc ->
   ps_na ## ps_acc ∪ accessible_in_trans_memory_pages i trans ->
@@ -46,8 +46,8 @@ Lemma ftlr_nop {i trans' mem_acc_tx ai regs ps_acc p_tx p_rx ps_na instr} trans 
                       RX_state@i:= a4 -∗
                       mailbox.rx_page i p_rx -∗
                       rx_pages (list_to_set list_of_vmids ∖ {[i]}) -∗
-                      (∃ trans, ▷ VMProp V0 (vmprop_zero i p_tx p_rx trans) (1 / 2)) -∗
-                      VMProp i (vmprop_unknown i p_tx p_rx a2) 1 -∗
+                      ▷ VMProp V0 (vmprop_zero i p_tx p_rx) (1 / 2)) -∗
+                      VMProp i (vmprop_unknown i p_tx p_rx) 1 -∗
                       transaction_pagetable_entries_owned i a3 -∗
                       pagetable_entries_excl_owned i (a1 ∖ {[p_rx; p_tx]} ∖ (accessible_in_trans_memory_pages i a3)) -∗
                       retrieval_entries_owned i a3 -∗
@@ -68,8 +68,8 @@ Lemma ftlr_nop {i trans' mem_acc_tx ai regs ps_acc p_tx p_rx ps_na instr} trans 
    RX_state@i:= rx_state -∗
    mailbox.rx_page i p_rx -∗
    rx_pages (list_to_set list_of_vmids ∖ {[i]}) -∗
-   (∃ trans, ▷ VMProp V0 (vmprop_zero i p_tx p_rx trans) (1 / 2)) -∗
-   VMProp i (vmprop_unknown i p_tx p_rx trans') 1 -∗
+   ▷ VMProp V0 (vmprop_zero i p_tx p_rx) (1 / 2)) -∗
+   VMProp i (vmprop_unknown i p_tx p_rx) 1 -∗
    transaction_pagetable_entries_owned i trans -∗
    pagetable_entries_excl_owned i (ps_acc ∖ {[p_rx; p_tx]} ∖ (accessible_in_trans_memory_pages i trans)) -∗
    retrieval_entries_owned i trans -∗
@@ -93,9 +93,8 @@ Lemma ftlr_nop {i trans' mem_acc_tx ai regs ps_acc p_tx p_rx ps_na instr} trans 
     iDestruct ("Hacc_regs" $! (ai ^+ 1)%f with "PC") as "[%Htotal_regs' regs]".
     iDestruct ("Hacc_mem_acc" with "[$mem_instr]") as "mem_acc_tx".
     iApply ("IH" $! _ _ ps_acc _ trans _ Htotal_regs' Hsubset_mb Hdisj_na Hnin_rx Hnin_tx with "regs tx pgt_tx pgt_acc pgt_acc'
-                       LB trans_hpool_global tran_pgt_transferred retri R0z R1z R2z rx_state rx other_rx [prop0] propi
+                       LB trans_hpool_global tran_pgt_transferred retri R0z R1z R2z rx_state rx other_rx prop0 propi
                            tran_pgt_owned pgt_owned retri_owned [mem_rest mem_acc_tx mem_tx]").
-    { iDestruct "prop0" as "[%x prop0]". iExists x. iFrame. }
     {
       iDestruct (memory_pages_split_singleton' p_tx ps_acc with "[mem_acc_tx $mem_tx]") as "mem_acc". set_solver + Hsubset_mb.
       iExists mem_acc_tx;by iFrame "mem_acc_tx".
